TM/Code/WriteValue.v
@@ -4,13 +4,21 @@ Require Import TM.Compound.WriteString.
 Require Import TMTac.
 
 
-Lemma WriteString_L_right (sig : Type) (str : list sig) t :
-  right (WriteString_Fun L t str) = rev str ++ right t.
+Lemma WriteString_L_local (sig : Type) (str : list sig) t :
+  str <> nil ->
+  tape_local (WriteString_Fun L t str) = rev str ++ right t.
 Proof.
-  revert t. induction str; intros; cbn in *.
+  revert t. induction str as [ | s [ | s' str'] IH]; intros; cbn in *.
+  - tauto.
   - reflexivity.
-  - rewrite IHstr. simpl_tape. rewrite <- app_assoc. reflexivity.
+  - rewrite IH. 2: congruence. simpl_tape. rewrite <- !app_assoc. reflexivity.
 Qed.
+
+Lemma tape_local_contains (sig : Type) (X : Type) (cX : codable sig X) (x : X) t :
+  tape_local t = inl START :: encode x ++ [inl STOP] ->
+  t ≃ x.
+Proof. intros -> % midtape_tape_local_cons. repeat econstructor. Qed.
+
 
 Arguments WriteString_Fun : simpl never.
 
@@ -18,49 +26,37 @@ Section WriteValue.
 
   Variable (sig: finType) (X: Type) (cX: codable sig X).
 
-  Definition WriteValue (x:X) : { M : mTM sig^+ 1 & states M -> unit } :=
-    WriteString L (inl STOP :: rev (encode x));; Write (inl START).
+  Definition WriteValue (str : list sig) : { M : mTM sig^+ 1 & states M -> unit } :=
+    WriteString L (rev (inl START :: map inr str ++ [inl STOP])).
 
-  Definition WriteValue_Rel (x : X) : Rel (tapes sig^+ 1) (unit * tapes sig^+ 1) :=
-    Mk_R_p (ignoreParam (fun tin tout => isRight tin -> tout ≃ x)).
+  Definition WriteValue_Rel (str : list sig) : Rel (tapes sig^+ 1) (unit * tapes sig^+ 1) :=
+    Mk_R_p (ignoreParam (fun tin tout => forall (x:X), encode x = str -> isRight tin -> tout ≃ x)).
 
-
-  Definition WriteValue_steps (x : X) := 5 + 3 * size cX x.
+  Definition WriteValue_steps (l : nat) := 3 + 2 * l.
   
-  Lemma WriteValue_Sem (x : X) :
-    WriteValue x ⊨c(WriteValue_steps x) WriteValue_Rel x.
+  Lemma WriteValue_Sem (str : list sig) :
+    WriteValue str ⊨c(WriteValue_steps (length str)) WriteValue_Rel str.
   Proof.
     unfold WriteValue_steps. eapply RealiseIn_monotone.
-    { unfold WriteValue. repeat TM_Correct. eapply WriteString_Sem. }
-    { cbn. rewrite rev_length, map_length. apply Nat.eq_le_incl. unfold size. omega. }
+    { unfold WriteValue. eapply WriteString_Sem. }
+    { unfold WriteString_steps. rewrite !rev_length. cbn [length]. rewrite app_length.
+      unfold size. cbn. rewrite map_length. omega. }
     {
-      intros tin ((), tout) H. intros HRight.
-      TMSimp; clear_trivial_eqs.
-      repeat econstructor. f_equal. rewrite WriteString_L_right. cbn.
-      rewrite <- app_assoc. rewrite rev_involutive. rewrite isRight_right; auto.
+      intros tin ((), tout) H. intros x <- HRight.
+      TMSimp; clear_trivial_eqs. eapply tape_local_contains. rewrite WriteString_L_local.
+      - rewrite rev_app_distr, <- !app_assoc, rev_involutive, <- !app_assoc. cbn. f_equal. f_equal. f_equal. now apply isRight_right.
+      - rewrite rev_app_distr, <- !app_assoc. cbn. congruence.
     }
   Qed.
 
 End WriteValue.
 
 
-Section Steps_comp.
-  Variable (sig tau: finType) (X:Type) (cX: codable sig X).
-  Variable (I : Retract sig tau).
-
-  Lemma WriteValue_steps_comp l :
-    WriteValue_steps (Encode_map cX I) l = WriteValue_steps cX l.
-  Proof. unfold WriteValue_steps. now rewrite Encode_map_hasSize. Qed.
-
-End Steps_comp.
-
-
-
 Ltac smpl_TM_WriteValue :=
   match goal with
-  | [ |- WriteValue _ _ ⊨ _ ] => eapply RealiseIn_Realise; apply WriteValue_Sem
-  | [ |- WriteValue _ _ ⊨c(_) _ ] => apply WriteValue_Sem
-  | [ |- projT1 (WriteValue _ _) ↓ _ ] => eapply RealiseIn_TerminatesIn; apply WriteValue_Sem
+  | [ |- WriteValue _ ⊨ _ ] => eapply RealiseIn_Realise; apply WriteValue_Sem
+  | [ |- WriteValue _ ⊨c(_) _ ] => apply WriteValue_Sem
+  | [ |- projT1 (WriteValue _) ↓ _ ] => eapply RealiseIn_TerminatesIn; apply WriteValue_Sem
   end.
 
 Smpl Add smpl_TM_WriteValue : TM_Correct.
