TM/Compound/WriteString.v
@@ -16,13 +16,15 @@ Section Write_String.
   Fixpoint WriteString (l : list sig) : pTM sig unit 1 :=
     match l with
     | [] => Nop
+    | [x] => Write x
     | x :: xs => WriteMove x D;; WriteString xs
     end.
 
   Fixpoint WriteString_Fun (sig' : Type) (t : tape sig') (str : list sig') :=
     match str with
     | nil => t
-    | s :: str' => WriteString_Fun (tape_move_mono t (Some s, D)) str'
+    | [x] => tape_write t (Some x)
+    | x :: str' => WriteString_Fun (tape_move_mono t (Some x, D)) str'
     end.
   
   Lemma Write_String_nil (sig' : Type) (t : tape sig') :
@@ -32,34 +34,49 @@ Section Write_String.
   Fixpoint WriteString_sem_fix (str : list sig) : pRel sig unit 1 :=
     match str with
     | nil => Nop_Rel
-    | s :: str' =>
-      WriteMove_Rel s D |_tt ∘ WriteString_sem_fix str'
+    | [x] => Write_Rel x
+    | x :: str' =>
+      WriteMove_Rel x D |_tt ∘ WriteString_sem_fix str'
     end.
+
+  Definition WriteString_steps l :=
+    2 * l - 1.
     
   Lemma WriteString_fix_Sem (str : list sig) :
-    WriteString str ⊨c(3 * |str|) (WriteString_sem_fix str).
+    WriteString str ⊨c(WriteString_steps (length str)) (WriteString_sem_fix str).
   Proof.
-    induction str; cbn; eapply RealiseIn_monotone; cbn.
-    - repeat TM_Correct.
-    - omega.
-    - firstorder.
-    - repeat TM_Correct.
-    - omega.
-    - intros tin (y, tout) H. TMSimp. exists tmid. repeat split; auto. 
+    induction str as [ | s [ | s' str'] IH ].
+    - cbn. change (2 * 0 - 1) with 0. repeat TM_Correct.
+    - cbn. change (2 * 1 - 1) with 1. repeat TM_Correct.
+    - change (WriteString (s :: s' :: str')) with (WriteMove s D;; WriteString (s' :: str')).
+      eapply RealiseIn_monotone.
+      { TM_Correct. TM_Correct. apply IH. }
+      { unfold WriteString_steps. cbn. omega. }
+      { intros t1 t3 H. destruct H as (()&t2&H1&H2).
+        change (WriteString_sem_fix (s :: s' :: str')) with (WriteMove_Rel s D |_tt ∘ WriteString_sem_fix (s' :: str')).
+        exists t2. split; auto.
+      }
   Qed.
   
+
   Definition WriteString_Rel str : Rel (tapes sig 1) (unit * tapes sig 1) :=
     Mono.Mk_R_p (ignoreParam (fun tin tout => tout = WriteString_Fun tin str)).
 
   Lemma WriteString_Sem str :
-    WriteString str ⊨c(3 * |str|) (WriteString_Rel str).
+    WriteString str ⊨c(WriteString_steps (length str)) (WriteString_Rel str).
   Proof.
-    eapply RealiseIn_monotone with (k1 := 3 * (|str|)).
-    - apply WriteString_fix_Sem.
-    - reflexivity.
-    - induction str as [ | s str' IH]; intros tin (yout, tout) H; cbn in *.
-      + now TMSimp.
-      + TMSimp; clear_trivial_eqs. hnf in IH. specialize IH with (1 := H0). now TMSimp.
+    eapply RealiseIn_monotone.
+    { apply WriteString_fix_Sem. }
+    { reflexivity. }
+    { induction str as [ | s [ | s' str'] IH]; intros tin (yout, tout) H.
+      - cbn. now TMSimp.
+      - cbn. now TMSimp.
+      - change (WriteString_sem_fix (s :: s' :: str')) with ((WriteMove_Rel s D |_tt ∘ WriteString_sem_fix (s' :: str'))) in H.
+        destruct H as (tmid&H1&H2). hnf in H1. apply IH in H2.
+        (* cbv [WriteString_Rel Mk_R_p ignoreParam].
+        change (WriteString_Fun tin[@Fin0] (s :: s' :: str')) with (WriteString_Fun (tape_move_mono tin[@Fin0] (Some s, D)) (s' :: str')). *)
+        now TMSimp.
+    }
   Qed.
 
 End Write_String.
